Semantics/IRStepThms.thy
@@ -94,18 +94,18 @@ proof (induction rule: "step.induct")
     by (metis is_AbstractEndNode.simps SequentialNode.hyps(1) is_sequential_node.simps(18,35)
         is_EndNode.elims(2) is_LoopEndNode_def)
   have notnew: "\<not>(is_NewInstanceNode (kind g nid))"
-    by (metis is_NewInstanceNode_def SequentialNode.hyps(1) is_sequential_node.simps(40))
+    by (metis is_NewInstanceNode_def SequentialNode.hyps(1) is_sequential_node.simps(41))
   have notload: "\<not>(is_LoadFieldNode (kind g nid))"
     by (metis is_LoadFieldNode_def SequentialNode.hyps(1) is_sequential_node.simps(33))
   have notstore: "\<not>(is_StoreFieldNode (kind g nid))"
-    by (metis is_StoreFieldNode_def SequentialNode.hyps(1) is_sequential_node.simps(52))
+    by (metis is_StoreFieldNode_def SequentialNode.hyps(1) is_sequential_node.simps(53))
   have notdivrem:  "\<not>(is_IntegerDivRemNode (kind g nid))"
-    by (metis is_IntegerDivRemNode.simps SequentialNode.hyps(1) is_sequential_node.simps(50,51)
+    by (metis is_IntegerDivRemNode.simps SequentialNode.hyps(1) is_sequential_node.simps(51,52)
         is_SignedDivNode_def is_SignedRemNode_def)
   from notif notend notnew notload notstore notdivrem
   show ?case
-    by (smt (verit) SequentialNode step.cases is_sequential_node.simps(14,20,50,51) Pair_inject
-        IRNode.discI(37) IRNode.disc(795,1527,2991))
+    by (smt (verit) SequentialNode Pair_inject IRNode.disc(870,1614,3102) IRNode.discI(38)
+        step.cases is_sequential_node.simps(12,14,20,40,51,52))
 next
   case (FixedGuardNode nid cond before "next" condE m p val h)
   have notseq: "\<not>(is_sequential_node (kind g nid))"
@@ -114,20 +114,8 @@ next
     by (simp add: FixedGuardNode.hyps(1))
   from notseq notend 
   show ?case
-    by (smt (verit) FixedGuardNode.hyps(1,5) IRNode.distinct(583,1287,1311,1333,1353,1355,1359)
-        step.cases Pair_inject IRNode.inject(12))
-next
-  case (IfNode nid cond tb fb m val "next" h)
-  then have notseq: "\<not>(is_sequential_node (kind g nid))"
-    by (simp add: IfNode.hyps(1))
-  have notend: "\<not>(is_AbstractEndNode (kind g nid))"
-    by (simp add: IfNode.hyps(1))
-  have notdivrem: "\<not>(is_IntegerDivRemNode (kind g nid))" 
-    by (simp add: IfNode.hyps(1))
-  from notseq notend notdivrem
-  show ?case
-    by (smt (verit) IRNode.inject(14) Pair_inject repDet evalDet IfNode.hyps step.cases
-        IRNode.distinct(587,1287,1493,1515,1535,1537,1541))
+    by (smt (verit) IRNode.distinct(373,703,1407,1431,1451,1453,1473,1475,1479) IRNode.inject(13)
+        step.cases Pair_inject FixedGuardNode.hyps(1,5))
 next
   case (BytecodeExceptionNode nid args st n' ex h' ref h m' m)
   have notseq: "\<not>(is_sequential_node (kind g nid))"
@@ -148,43 +136,116 @@ next
     by (simp add: BytecodeExceptionNode.hyps(1))
   have notend: "\<not>(is_AbstractEndNode (kind g nid))"
     by (simp add: BytecodeExceptionNode.hyps(1))
-  from notseq notif notref notnew notload notstore notdivrem notfixedguard notend
+  have notnewarray: "\<not>(is_NewArrayNode (kind g nid))"
+    by (simp add: BytecodeExceptionNode.hyps(1))
+  from notseq notif notref notnew notload notstore notdivrem notfixedguard notend notnewarray
   show ?case
-    by (smt (verit) BytecodeExceptionNode.hyps IRNode.disc(673,1527,2991) IRNode.inject(6) repDet
-        IRNode.discI(14,37) IRNode.distinct(653,655) Pair_inject step.cases)
+    by (smt (verit) BytecodeExceptionNode.hyps IRNode.disc(1614,3102) IRNode.inject(7) repDet
+        IRNode.discI(13,15,38) IRNode.distinct(359,751,773,775) Pair_inject step.cases)
+next
+  case (IfNode nid cond tb fb m val "next" h)
+  then have notseq: "\<not>(is_sequential_node (kind g nid))"
+    by (simp add: IfNode.hyps(1))
+  have notend: "\<not>(is_AbstractEndNode (kind g nid))"
+    by (simp add: IfNode.hyps(1))
+  have notdivrem: "\<not>(is_IntegerDivRemNode (kind g nid))"
+    by (simp add: IfNode.hyps(1))
+  have notnewarray: "\<not>(is_NewArrayNode (kind g nid))"
+    by (simp add: IfNode.hyps(1))
+  from notseq notend notdivrem notnewarray
+  show ?case
+    by (smt (verit) IRNode.inject(15) Pair_inject repDet evalDet IfNode.hyps step.cases
+        IRNode.distinct(377,707,1407,1613,1633,1635,1655,1657,1661))
 next
   case (EndNodes nid merge i phis inputs m vs m' h)
   have notseq: "\<not>(is_sequential_node (kind g nid))"
     by (metis is_EndNode.elims(2) is_LoopEndNode_def is_sequential_node.simps(18,35)
         is_AbstractEndNode.simps EndNodes.hyps(1))
   have notif: "\<not>(is_IfNode (kind g nid))"
-    by (metis IRNode.distinct_disc(1499) is_AbstractEndNode.elims(2) EndNodes.hyps(1) is_IfNode_def
-        is_EndNode.simps(15))
+    by (metis IRNode.distinct_disc(1620) is_AbstractEndNode.elims(2) EndNodes.hyps(1) is_IfNode_def
+        is_EndNode.simps(16))
   have notref: "\<not>(is_RefNode (kind g nid))"
     by (metis notseq is_RefNode_def is_sequential_node.simps(7))
   have notnew: "\<not>(is_NewInstanceNode (kind g nid))"
-    by (metis IRNode.distinct_disc(2626) is_EndNode.simps(38) is_NewInstanceNode_def
+    by (metis IRNode.distinct_disc(2746) is_EndNode.simps(39) is_NewInstanceNode_def
         is_AbstractEndNode.simps EndNodes.hyps(1))
   have notload: "\<not>(is_LoadFieldNode (kind g nid))"
-    by (metis IRNode.distinct_disc(2424) is_EndNode.simps(27) is_LoadFieldNode_def EndNodes.hyps(1)
+    by (metis IRNode.distinct_disc(2544) is_EndNode.simps(28) is_LoadFieldNode_def EndNodes.hyps(1)
         is_AbstractEndNode.simps)
   have notstore: "\<not>(is_StoreFieldNode (kind g nid))"
-    by (metis IRNode.distinct_disc(2652) is_EndNode.simps(51) is_StoreFieldNode_def EndNodes.hyps(1)
+    by (metis IRNode.distinct_disc(2772) is_EndNode.simps(52) is_StoreFieldNode_def EndNodes.hyps(1)
         is_AbstractEndNode.simps)
   have notdivrem: "\<not>(is_IntegerDivRemNode (kind g nid))"
     using EndNodes.hyps(1) is_SignedDivNode_def is_SignedRemNode_def by auto
   have notfixedguard: "\<not>(is_FixedGuardNode (kind g nid))"
-    by (metis IRNode.distinct_disc(1317) is_EndNode.simps(13) is_FixedGuardNode_def EndNodes.hyps(1)
+    by (metis IRNode.distinct_disc(1437) is_EndNode.simps(14) is_FixedGuardNode_def EndNodes.hyps(1)
         is_AbstractEndNode.simps)
   have notbytecodeexception: "\<not>(is_BytecodeExceptionNode (kind g nid))"
-    by (metis IRNode.distinct_disc(617) is_BytecodeExceptionNode_def is_AbstractEndNode.simps
-        is_EndNode.simps(7) EndNodes.hyps(1))
+    by (metis IRNode.distinct_disc(738) is_BytecodeExceptionNode_def is_AbstractEndNode.simps
+        is_EndNode.simps(8) EndNodes.hyps(1))
+  have notnewarray: "\<not>(is_NewArrayNode (kind g nid))"
+    by (metis IRNode.distinct_disc(2743) is_EndNode.simps(38) is_NewArrayNode_def EndNodes.hyps(1)
+        is_AbstractEndNode.simps)
+  have notarraylength: "\<not>(is_ArrayLengthNode (kind g nid))"
+    by (metis IRNode.distinct_disc(407) is_EndNode.simps(5) is_ArrayLengthNode_def EndNodes.hyps(1)
+        is_AbstractEndNode.simps)
   from notseq notif notref notnew notload notstore notdivrem notfixedguard notbytecodeexception
+       notnewarray notarraylength
   show ?case
     by (smt (verit) is_FixedGuardNode_def repAllDet evalAllDet is_IfNode_def EndNodes step.cases
         is_RefNode_def Pair_inject is_LoadFieldNode_def is_NewInstanceNode_def is_StoreFieldNode_def
-        is_SignedDivNode_def is_SignedRemNode_def is_IntegerDivRemNode.elims(3)
-        is_BytecodeExceptionNode_def)
+        is_SignedDivNode_def is_SignedRemNode_def is_IntegerDivRemNode.elims(3) is_NewArrayNode_def
+        is_BytecodeExceptionNode_def is_ArrayLengthNode_def)
+next
+  case (NewArrayNode nid len st n' lenE m length' arrayType h' ref h refNo h'')
+  have notseq: "\<not>(is_sequential_node (kind g nid))"
+    by (simp add: NewArrayNode.hyps(1))
+  have notend: "\<not>(is_AbstractEndNode (kind g nid))"
+    by (simp add: NewArrayNode.hyps(1))
+  have notif: "\<not>(is_IfNode (kind g nid))"
+    by (simp add: NewArrayNode.hyps(1))
+  have notload: "\<not>(is_LoadFieldNode (kind g nid))"
+    by (simp add: NewArrayNode.hyps(1))
+  have notstore: "\<not>(is_StoreFieldNode (kind g nid))"
+    by (simp add: NewArrayNode.hyps(1))
+  have notfixedguard: "\<not>(is_FixedGuardNode (kind g nid))"
+    by (simp add: NewArrayNode.hyps(1))
+  have notbytecodeexception: "\<not>(is_BytecodeExceptionNode (kind g nid))"
+    by (simp add: NewArrayNode.hyps(1))
+  have notarraylength: "\<not>(is_ArrayLengthNode (kind g nid))"
+    by (simp add: NewArrayNode.hyps(1))
+  have notnew: "\<not>(is_NewInstanceNode (kind g nid))"
+    by (simp add: NewArrayNode.hyps(1))
+  from notseq notend notif notload notstore notfixedguard notbytecodeexception notarraylength notnew
+  show ?case
+    by (smt (verit) IRNode.discI(27) repDet evalDet Value.inject(2) IRNode.distinct(3131,3129)
+        is_FixedGuardNode_def is_NewInstanceNode_def is_ArrayLengthNode_def is_IfNode_def
+        is_BytecodeExceptionNode_def is_StoreFieldNode_def IRNode.inject EndNodes evalAllDet
+        Pair_inject step.cases NewArrayNode)
+next
+  case (ArrayLengthNode nid x nid' xE m ref h arrayVal length' m')
+  have notseq: "\<not>(is_sequential_node (kind g nid))"
+    by (simp add: ArrayLengthNode.hyps(1))
+  have notend: "\<not>(is_AbstractEndNode (kind g nid))"
+    by (simp add: ArrayLengthNode.hyps(1))
+  have notif: "\<not>(is_IfNode (kind g nid))"
+    by (simp add: ArrayLengthNode.hyps(1))
+  have notstore: "\<not>(is_StoreFieldNode (kind g nid))"
+    by (simp add: ArrayLengthNode.hyps(1))
+  have notfixedguard: "\<not>(is_FixedGuardNode (kind g nid))"
+    by (simp add: ArrayLengthNode.hyps(1))
+  have notbytecodeexception: "\<not>(is_BytecodeExceptionNode (kind g nid))"
+    by (simp add: ArrayLengthNode.hyps(1))
+  have notnew: "\<not>(is_NewInstanceNode (kind g nid))"
+    by (simp add: ArrayLengthNode.hyps(1))
+  have notnewarray: "\<not>(is_NewArrayNode (kind g nid))"
+    by (simp add: ArrayLengthNode.hyps(1))
+  from notseq notend notif  notstore notfixedguard notbytecodeexception notnew notnewarray
+  show ?case
+    by (smt (verit) IRNode.disc(211,221,232,233) Value.inject(2) ArrayLengthNode step.cases evalDet
+        Pair_inject IRNode.inject is_StoreFieldNode_def is_BytecodeExceptionNode_def is_IfNode_def
+        is_ArrayLengthNode_def is_NewInstanceNode_def is_FixedGuardNode_def is_NewArrayNode_def
+        repDet)
 next
   case (NewInstanceNode nid f obj nxt h' ref h m' m)
   then have notseq: "\<not>(is_sequential_node (kind g nid))"
@@ -201,10 +262,14 @@ next
     by (simp add: NewInstanceNode.hyps(1))
   have notdivrem:  "\<not>(is_IntegerDivRemNode (kind g nid))"
     by (simp add: NewInstanceNode.hyps(1))
-  from notseq notend notif notref notload notstore notdivrem
+  have notnewarray:  "\<not>(is_NewArrayNode (kind g nid))"
+    by (simp add: NewInstanceNode.hyps(1))
+  have notarraylength:  "\<not>(is_ArrayLengthNode (kind g nid))"
+    by (simp add: NewInstanceNode.hyps(1))
+  from notseq notend notif notref notload notstore notdivrem notnewarray notarraylength
   show ?case
-    by (smt (verit) NewInstanceNode step.cases IRNode.disc(1527,2991) IRNode.discI(14) Pair_inject
-        IRNode.distinct(633,1333,3053,3055) IRNode.inject(35,36,37))
+    by (smt (verit) NewInstanceNode step.cases IRNode.disc(1614,2234,3102) IRNode.discI(4,15)
+        Pair_inject IRNode.distinct(753,1453,3173,3175) IRNode.inject(38))
 next
   case (LoadFieldNode nid f obj nxt m ref h v m')
   then have notseq: "\<not>(is_sequential_node (kind g nid))"
@@ -215,8 +280,9 @@ next
     by (simp add: LoadFieldNode.hyps(1))
   from notseq notend notdivrem
   show ?case
-    by (smt (verit) LoadFieldNode step.cases evalDet IRNode.inject(26) option.discI option.inject
-        IRNode.distinct(611,1311,1493,2439,2459,2461,2465) Pair_inject Value.inject(2) repDet)
+    by (smt (verit) LoadFieldNode step.cases evalDet IRNode.inject(27) option.discI option.inject
+        IRNode.distinct(401,731,1431,1613,2557,2559,2579,2581,2585) Pair_inject Value.inject(2)
+        repDet)
 next
   case (StaticLoadFieldNode nid f nxt h v m' m)
   then have notseq: "\<not>(is_sequential_node (kind g nid))"
@@ -227,8 +293,8 @@ next
     by (simp add: StaticLoadFieldNode.hyps(1))
   from notseq notend notdivrem
   show ?case
-    by (smt (verit) IRNode.distinct(611,1311,1493,2439,2459,2461,2465) IRNode.inject(26) step.cases
-        StaticLoadFieldNode Pair_inject option.distinct(1))
+    by (smt (verit) IRNode.distinct(401,731,1431,1613,2557,2559,2579,2581,2585) IRNode.inject(27)
+        step.cases StaticLoadFieldNode Pair_inject option.distinct(1))
 next
   case (StoreFieldNode nid f newval uu obj nxt m val ref h' h m')
   then have notseq: "\<not>(is_sequential_node (kind g nid))"
@@ -239,8 +305,9 @@ next
     by (simp add: StoreFieldNode.hyps(1))
   from notseq notend notdivrem
   show ?case
-    by (smt (verit) IRNode.distinct(659,1359,1541,2465,3059,3389,3411) IRNode.inject(50) step.cases
-        StoreFieldNode repDet evalDet option.discI Pair_inject Value.inject(2) option.inject)
+    by (smt (verit) IRNode.distinct(449,779,1479,1661,2585,3135,3179,3509,3531) IRNode.inject(51)
+        step.cases StoreFieldNode evalDet option.discI Pair_inject Value.inject(2) option.inject
+        repDet)
 next
   case (StaticStoreFieldNode nid f newval uv nxt m val h' h m')
   then have notseq: "\<not>(is_sequential_node (kind g nid))"
@@ -251,8 +318,9 @@ next
     by (simp add: StaticStoreFieldNode.hyps(1))
   from notseq notend notdivrem
   show ?case
-    by (smt (verit) IRNode.distinct(659,1359,1541,2465,3059,3389,3411) IRNode.inject(50) step.cases
-        StoreFieldNode repDet StaticStoreFieldNode.hyps option.distinct(1) Pair_inject evalDet)
+    by (smt (verit) IRNode.distinct(449,779,1479,1661,2585,3135,3179,3509,3531) IRNode.inject(51)
+        step.cases StoreFieldNode StaticStoreFieldNode.hyps option.distinct(1) Pair_inject evalDet
+        repDet)
 next
   case (SignedDivNode nid x y zero sb nxt m v1 v2 v m' h)
   then have notseq: "\<not>(is_sequential_node (kind g nid))"
@@ -261,8 +329,8 @@ next
     by (simp add: SignedDivNode.hyps(1))
   from notseq notend
   show ?case
-    by (smt (verit) IRNode.distinct(653,1353,1535,2459,3053,3385,3389) IRNode.inject(47) step.cases
-        SignedDivNode repDet evalDet Pair_inject)
+    by (smt (verit) IRNode.distinct(443,773,1473,1655,2579,3129,3173,3505,3509) IRNode.inject(48)
+        step.cases SignedDivNode repDet evalDet Pair_inject)
 next
   case (SignedRemNode nid x y zero sb nxt m v1 v2 v m' h)
   then have notseq: "\<not>(is_sequential_node (kind g nid))"
@@ -271,8 +339,8 @@ next
     by (simp add: SignedRemNode.hyps(1))
   from notseq notend
   show ?case
-    by (smt (verit) IRNode.distinct(655,1355,1537,2461,3055,3385,3411) IRNode.inject(48) step.cases
-        SignedRemNode repDet evalDet Pair_inject)
+    by (smt (verit) IRNode.distinct(445,775,1475,1657,2581,3131,3175,3505,3531) IRNode.inject(49)
+        step.cases SignedRemNode repDet evalDet Pair_inject)
 qed
 
 lemma stepRefNode:
@@ -301,7 +369,7 @@ lemma step_in_ids:
   assumes "g, p \<turnstile> (nid, m, h) \<rightarrow> (nid', m', h')"
   shows "nid \<in> ids g"
   using assms apply (induct "(nid, m, h)" "(nid', m', h')" rule: step.induct) apply fastforce
-  by (metis IRNode.distinct(675,1375,1557,2481,3075,3405,3427,3465) IRNode.disc(1739) ids_some
-      is_EndNode.simps(59) is_AbstractEndNode.simps not_in_g)+
+  by (metis IRNode.distinct(465,795,1495,1677,2601,3151,3195,3547,3525,3585) IRNode.disc(1829)
+      is_EndNode.simps(60) is_AbstractEndNode.simps not_in_g)+
 
 end
